record position within input stream

src/3d/prelude/EverParse3d.Actions.fst
@@ -27,7 +27,28 @@ module LP = LowParse.Spec.Base
 module LPL = LowParse.Low.Base
 
 unfold
-let valid_len
+let valid_consumed
+  (#input_buffer_t: Type0)
+  (# [tcresolve ()] inst : I.input_stream_inst input_buffer_t)
+  (#k: LP.parser_kind)
+  (#t: Type)
+  (p: LP.parser k t)
+  (h: HS.mem)
+  (h': HS.mem)
+  (sl: input_buffer_t)
+: Tot prop
+= I.live sl h /\
+  I.live sl h' /\
+  begin
+    let s = I.get_remaining sl h in
+    begin match LP.parse p s with
+    | None -> False
+    | Some (_, len) -> I.get_remaining sl h' == Seq.slice s len (Seq.length s)
+    end
+  end
+
+unfold
+let valid_length
   (#input_buffer_t: Type0)
   (# [tcresolve ()] inst : I.input_stream_inst input_buffer_t)
   (#k: LP.parser_kind)
@@ -35,7 +56,7 @@ let valid_len
   (p: LP.parser k t)
   (h: HS.mem)
   (sl: input_buffer_t)
-  (len: nat)
+  (len: int)
 : Tot prop
 = I.live sl h /\
   begin
@@ -62,15 +83,13 @@ let validate_with_action_t' (#k:LP.parser_kind) (#t:Type) (p:LP.parser k t) (inv
   (#input_buffer_t: Type0) ->
   (# [tcresolve ()] inst : I.input_stream_inst input_buffer_t) ->
   (sl: input_buffer_t) ->
-  (startPosition: U64.t) ->
   Stack U64.t
   (requires fun h ->
     I.live sl h /\
     inv (I.footprint sl) h /\
     loc_not_unused_in h `loc_includes` l /\
     address_liveness_insensitive_locs `loc_includes` l /\
-    l `loc_disjoint` I.footprint sl /\
-    U64.v startPosition + Seq.length (I.get_remaining sl h) == I.length_all #_ #inst sl
+    l `loc_disjoint` I.footprint sl
   )
   (ensures fun h res h' ->
     I.live sl h' /\
@@ -80,10 +99,10 @@ let validate_with_action_t' (#k:LP.parser_kind) (#t:Type) (p:LP.parser k t) (inv
     begin if LPE.is_success res
     then
       let s = I.get_remaining sl h in
-      let len = U64.v res - U64.v startPosition in
-      len >= 0 /\
-      valid_len p h sl len /\
-      I.get_remaining sl h' == (if allow_reading then s else Seq.slice s len (Seq.length s))
+      begin if allow_reading
+      then valid_length p h sl (U64.v res) /\ I.get_remaining sl h' == s
+      else valid_consumed p h h' sl
+      end
     else
       True
     end
@@ -134,10 +153,10 @@ let validate_with_success_action' (name: string) #nz #wk (#k1:parser_kind nz wk)
                          (v1:validate_with_action_t p1 inv1 l1 ar)
                          (#inv2:_) (#l2:eloc) #b (a:action p1 inv2 l2 b bool)
   : validate_with_action_t p1 (conj_inv inv1 inv2) (l1 `eloc_union` l2) ar
-  = fun input startPosition ->
+  = fun input ->
     let h0 = HST.get () in
-    [@(rename_let ("positionAfter" ^ name))]
-    let pos1 = v1 input startPosition in
+    [@(rename_let ("resultAfter" ^ name))]
+    let pos1 = v1 input in
     let h1 = HST.get () in
     modifies_address_liveness_insensitive_unused_in h0 h1;
     if LPL.is_success pos1
@@ -155,12 +174,12 @@ noextract
 let validate_drop_true
    (#k:LP.parser_kind) (#t:Type) (#p:LP.parser k t) (#inv:slice_inv) (#l:eloc) (v: validate_with_action_t' p inv l true)
 : Tot (validate_with_action_t' p inv l false)
-= fun input startPosition ->
-  let res = v input startPosition in
+= fun input ->
+  let res = v input in
   if LPE.is_success res
   then begin
     let h1 = HST.get () in
-    I.skip input (LPE.uint64_to_uint32 (res `U64.sub` startPosition));
+    I.skip input (LPE.uint64_to_uint32 res);
     let h2 = HST.get () in
     assert (h2 `extends` h1)
   end;
@@ -184,16 +203,16 @@ let validate_with_error_action' (name: string) #nz #wk (#k1:parser_kind nz wk) #
                          (v1:validate_with_action_t p1 inv1 l1 ar)
                          (#inv2:_) (#l2:eloc) (a:action p1 inv2 l2 false bool)
   : validate_with_action_t p1 (conj_inv inv1 inv2) (l1 `eloc_union` l2) ar
-  = fun input startPosition ->
+  = fun input ->
     let h0 = HST.get () in
-    [@(rename_let ("positionAfter" ^ name))]
-    let pos1 = v1 input startPosition in
+    [@(rename_let ("resultAfter" ^ name))]
+    let pos1 = v1 input in
     let h1 = HST.get () in
     modifies_address_liveness_insensitive_unused_in h0 h1;
     if LPL.is_success pos1
     then pos1
     else
-         [@(rename_let ("action_error_" ^ name))]
+         [@(rename_let ("actionError" ^ name))]
          let b = a input in
          if not b then validator_error_action_failed else pos1
 
@@ -204,8 +223,8 @@ let validate_with_error_action
 inline_for_extraction noextract
 let validate_ret
   : validate_with_action_t (parse_ret ()) true_inv eloc_none true
-  = fun input startPosition ->
-    startPosition
+  = fun input ->
+    0uL
 
 #push-options "--z3rlimit 16"
 
@@ -219,18 +238,18 @@ let validate_pair
        #nz2 #wk2 (#k2:parser_kind nz2 wk2) #t2 (#p2:parser k2 t2)
        (#inv2:_) (#l2:eloc) (#ar2:_) (v2:validate_with_action_t p2 inv2 l2 ar2)
   : validate_with_action_t (p1 `parse_pair` p2) (conj_inv inv1 inv2) (l1 `eloc_union` l2) false
-  = fun input startPosition ->
+  = fun input ->
     let h = HST.get () in
     LPC.nondep_then_eq p1 p2 (I.get_remaining input h);
-    [@(rename_let ("positionAfter" ^ name1))]
-    let pos1 = validate_drop v1 input startPosition in
+    [@(rename_let ("resultAfter" ^ name1))]
+    let pos1 = validate_drop v1 input in
     let h1 = HST.get () in
     modifies_address_liveness_insensitive_unused_in h h1;
     if LPL.is_error pos1
     then
       pos1
     else
-      validate_drop v2 input pos1
+      validate_drop v2 input
 
 inline_for_extraction noextract
 let validate_dep_pair
@@ -240,11 +259,11 @@ let validate_dep_pair
       #nz2 #wk2 (#k2:parser_kind nz2 wk2) (#t2:t1 -> Type) (#p2:(x:t1 -> parser k2 (t2 x)))
       #inv2 #l2 #ar2 (v2:(x:t1 -> validate_with_action_t (p2 x) inv2 l2 ar2))
   : Tot (validate_with_action_t (p1 `parse_dep_pair` p2) (conj_inv inv1 inv2) (l1 `eloc_union` l2) false)
-  = fun input startPosition ->
+  = fun input ->
       let h = HST.get () in
       LPC.parse_dtuple2_eq p1 p2 (I.get_remaining input h);
-      [@(rename_let ("positionAfter" ^ name1))]
-      let pos1 = v1 input startPosition in
+      [@(rename_let ("resultAfter" ^ name1))]
+      let pos1 = v1 input in
       let h1 = HST.get() in
       if LPL.is_error pos1
       then begin
@@ -255,7 +274,7 @@ let validate_dep_pair
         let x = r1 input in
         let h15 = HST.get () in
         let _ = modifies_address_liveness_insensitive_unused_in h h15 in
-        validate_drop (v2 x) input pos1
+        validate_drop (v2 x) input
 
 inline_for_extraction noextract
 let validate_dep_pair_with_refinement_and_action'
@@ -273,12 +292,17 @@ let validate_dep_pair_with_refinement_and_action'
              (l1 `eloc_union` (l1' `eloc_union` l2))
              false)
   =
-  fun input startPosition ->
+  fun input ->
       let h0 = HST.get () in
+      let startPosition = I.get_read_count input in
+      let startPosition = Cast.uint32_to_uint64 startPosition in
+      let h05 = HST.get () in
+      assert (h05 `extends` h0);
+      modifies_address_liveness_insensitive_unused_in h0 h05;
       LPC.parse_dtuple2_eq' #_ #_ (p1 `LPC.parse_filter` f) #_ #t2 p2 (I.get_remaining input h0);
       LPC.parse_filter_eq p1 f (I.get_remaining input h0);
-      [@(rename_let ("positionAfter" ^ name1))]
-      let res = v1 input startPosition in
+      [@(rename_let ("resultAfter" ^ name1))]
+      let res = v1 input in
       let h1 = HST.get() in
       modifies_address_liveness_insensitive_unused_in h0 h1;
       if LPL.is_error res
@@ -291,13 +315,13 @@ let validate_dep_pair_with_refinement_and_action'
         let field_value = r1 input in
         [@(rename_let (name1 ^ "ConstraintIsOk"))]
         let ok = f field_value in
-        [@(rename_let ("pos_or_error_after_" ^ name1))]
+        [@(rename_let ("resultAfter" ^ name1))]
         let res1 = check_constraint_ok_with_field_id ok startPosition res id1 in
+        let h2 = HST.get() in
         if LPL.is_error res1
         then
           res1
-        else
-             let h2 = HST.get() in
+        else begin
              modifies_address_liveness_insensitive_unused_in h1 h2;
              if not (a field_value input)
              then (LPL.set_validator_error_pos_and_code validator_error_action_failed startPosition id1) //action failed
@@ -305,9 +329,10 @@ let validate_dep_pair_with_refinement_and_action'
                let open LPL in
                let h15 = HST.get () in
                let _ = modifies_address_liveness_insensitive_unused_in h0 h15 in
-               validate_drop (v2 field_value) input res1
+               validate_drop (v2 field_value) input
              end
         end
+      end
 
 inline_for_extraction noextract
 let validate_dep_pair_with_refinement_and_action_total_zero_parser'
@@ -330,8 +355,13 @@ let validate_dep_pair_with_refinement_and_action_total_zero_parser'
            k1.parser_kind_metadata == Some ParserKindMetadataTotal
          ))
          (ensures (fun _ -> True))
-  = fun input startPosition ->
+  = fun input ->
       let h0 = HST.get () in
+      let startPosition = I.get_read_count input in
+      let startPosition = Cast.uint32_to_uint64 startPosition in
+      let h05 = HST.get () in
+      assert (h05 `extends` h0);
+      modifies_address_liveness_insensitive_unused_in h0 h05;
       LPC.parse_dtuple2_eq' #_ #_ (p1 `LPC.parse_filter` f) #_ #t2 p2 (I.get_remaining input h0);
       LPC.parse_filter_eq p1 f (I.get_remaining input h0);
       [@inline_let] let _ = LP.parser_kind_prop_equiv k1 p1 in
@@ -341,7 +371,7 @@ let validate_dep_pair_with_refinement_and_action_total_zero_parser'
         let field_value = r1 input in
         [@(rename_let (name1 ^ "ConstraintIsOk"))]
         let ok = f field_value in
-        [@(rename_let ("pos_or_error_after_" ^ name1))]
+        [@(rename_let ("resultAfter" ^ name1))]
         let res1 = check_constraint_ok_with_field_id ok startPosition startPosition id1 in
         if LPL.is_error res1
         then
@@ -354,7 +384,7 @@ let validate_dep_pair_with_refinement_and_action_total_zero_parser'
                let open LPL in
                let h15 = HST.get () in
                let _ = modifies_address_liveness_insensitive_unused_in h0 h15 in
-               validate_drop (v2 field_value) input res1
+               validate_drop (v2 field_value) input
              end
         end
 
@@ -395,10 +425,10 @@ let validate_dep_pair_with_action
              (conj_inv inv1 (conj_inv inv1' inv2))
              (l1 `eloc_union` (l1' `eloc_union` l2))
              false)
-  = fun input startPosition ->
+  = fun input ->
       let h0 = HST.get () in
       LPC.parse_dtuple2_eq' #_ #_ p1 #_ #t2 p2 (I.get_remaining input h0);
-      let res = v1 input startPosition in
+      let res = v1 input in
       let h1 = HST.get() in
       modifies_address_liveness_insensitive_unused_in h0 h1;
       if LPL.is_error res
@@ -416,7 +446,7 @@ let validate_dep_pair_with_action
                let open LPL in
                let h15 = HST.get () in
                let _ = modifies_address_liveness_insensitive_unused_in h0 h15 in
-               validate_drop (v2 field_value) input res
+               validate_drop (v2 field_value) input
              end
       end
 
@@ -434,12 +464,17 @@ let validate_dep_pair_with_refinement'
              (conj_inv inv1 inv2)
              (l1 `eloc_union` l2)
              false)
-  = fun input startPosition ->
+  = fun input ->
       let h0 = HST.get () in
+      let startPosition = I.get_read_count input in
+      let startPosition = Cast.uint32_to_uint64 startPosition in
+      let h05 = HST.get () in
+      assert (h05 `extends` h0);
+      modifies_address_liveness_insensitive_unused_in h0 h05;
       LPC.parse_dtuple2_eq' #_ #_ (p1 `LPC.parse_filter` f) #_ #t2 p2 (I.get_remaining input h0);
       LPC.parse_filter_eq p1 f (I.get_remaining input h0);
-      [@(rename_let ("positionAfter" ^ name1))]
-      let res = v1 input startPosition in
+      [@(rename_let ("resultAfter" ^ name1))]
+      let res = v1 input in
       let h1 = HST.get() in
       modifies_address_liveness_insensitive_unused_in h0 h1;
       if LPL.is_error res
@@ -451,7 +486,7 @@ let validate_dep_pair_with_refinement'
         let field_value = r1 input in
         [@(rename_let (name1 ^ "ConstraintIsOk"))]
         let ok = f field_value in
-        [@(rename_let ("positionOrErrorAfter" ^ name1))]
+        [@(rename_let ("resultAfter" ^ name1))]
         let res1 = check_constraint_ok_with_field_id ok startPosition res id1 in
         if LPL.is_error res1
         then
@@ -465,7 +500,7 @@ let validate_dep_pair_with_refinement'
              // assert (valid_pos (p1 `(LPC.parse_filter #k1 #t1)` f) h0 input (uint64_to_uint32 pos) (uint64_to_uint32 res));
              let h15 = HST.get () in
              let _ = modifies_address_liveness_insensitive_unused_in h0 h15 in
-             validate_drop (v2 field_value) input res1
+             validate_drop (v2 field_value) input
         end
 
 inline_for_extraction noextract
@@ -488,8 +523,13 @@ let validate_dep_pair_with_refinement_total_zero_parser'
            k1.parser_kind_metadata == Some ParserKindMetadataTotal
          ))
          (ensures (fun _ -> True))
-  = fun input startPosition ->
+  = fun input ->
       let h0 = HST.get () in
+      let startPosition = I.get_read_count input in
+      let startPosition = Cast.uint32_to_uint64 startPosition in
+      let h05 = HST.get () in
+      assert (h05 `extends` h0);
+      modifies_address_liveness_insensitive_unused_in h0 h05;
       LPC.parse_dtuple2_eq' #_ #_ (p1 `LPC.parse_filter` f) #_ #t2 p2 (I.get_remaining input h0);
       LPC.parse_filter_eq p1 f (I.get_remaining input h0);
       [@inline_let] let _ = LP.parser_kind_prop_equiv k1 p1 in
@@ -499,7 +539,7 @@ let validate_dep_pair_with_refinement_total_zero_parser'
         let field_value = r1 input in
         [@(rename_let (name1 ^ "ConstraintIsOk"))]
         let ok = f field_value in
-        [@(rename_let ("positionOrErrorAfter" ^ name1))]
+        [@(rename_let ("resultAfter" ^ name1))]
         let res1 = check_constraint_ok_with_field_id ok startPosition startPosition id1 in
         if LPL.is_error res1
         then res1
@@ -512,7 +552,7 @@ let validate_dep_pair_with_refinement_total_zero_parser'
              // assert (valid_pos (p1 `(LPC.parse_filter #k1 #t1)` f) h0 input (uint64_to_uint32 pos) (uint64_to_uint32 res));
              let h15 = HST.get () in
              let _ = modifies_address_liveness_insensitive_unused_in h0 h15 in
-             validate_drop (v2 field_value) input res1
+             validate_drop (v2 field_value) input
         end
 
 inline_for_extraction noextract
@@ -543,11 +583,11 @@ let validate_filter (name: string) #nz (#k:parser_kind nz _) (#t:_) (#p:parser k
                     #inv #l (v:validate_with_action_t p inv l true)
                     (r:leaf_reader p) (f:t -> bool) (cr:string) (cf:string)
   : Tot (validate_with_action_t #nz #WeakKindStrongPrefix (p `LPC.parse_filter` f) inv l false)
-  = fun input startPosition ->
+  = fun input ->
     let h = HST.get () in
     LPC.parse_filter_eq p f (I.get_remaining input h);
-    [@(rename_let ("positionAfter" ^ name))]
-    let res = v input startPosition in
+    [@(rename_let ("resultAfter" ^ name))]
+    let res = v input in
     let h1 = HST.get () in
     if LPL.is_error res
     then res
@@ -562,7 +602,6 @@ let validate_filter (name: string) #nz (#k:parser_kind nz _) (#t:_) (#p:parser k
       check_constraint_ok ok res
     end
 
-
 inline_for_extraction noextract
 let validate_filter_with_action
                     (name: string) #nz (#k:parser_kind nz _) (#t:_) (#p:parser k t)
@@ -570,11 +609,11 @@ let validate_filter_with_action
                     (r:leaf_reader p) (f:t -> bool) (cr:string) (cf:string)
                     (#b:bool) #inva (#la:eloc) (a: t -> action #nz #WeakKindStrongPrefix #(filter_kind k) #_ (p `LPC.parse_filter` f) inva la b bool)
   : Tot (validate_with_action_t #nz #WeakKindStrongPrefix (p `LPC.parse_filter` f) (conj_inv inv inva) (eloc_union l la) false)
-  = fun input startPosition ->
+  = fun input ->
     let h = HST.get () in
     LPC.parse_filter_eq p f (I.get_remaining input h);
-    [@(rename_let ("positionAfter" ^ name))]
-    let res = v input startPosition in
+    [@(rename_let ("resultAfter" ^ name))]
+    let res = v input in
     let h1 = HST.get () in
     if LPL.is_error res
     then res
@@ -602,10 +641,10 @@ let validate_with_dep_action
                     (r:leaf_reader p)
                     (#b:bool) #inva (#la:eloc) (a: t -> action p inva la b bool)
   : Tot (validate_with_action_t #nz p (conj_inv inv inva) (eloc_union l la) false)
-  = fun input startPosition ->
+  = fun input ->
     let h = HST.get () in
-    [@(rename_let ("positionAfter" ^ name))]
-    let res = v input startPosition in
+    [@(rename_let ("resultAfter" ^ name))]
+    let res = v input in
     let h1 = HST.get () in
     if LPL.is_error res
     then res
@@ -624,9 +663,8 @@ let validate_weaken #nz #wk (#k:parser_kind nz wk) #t (#p:parser k t)
                     #inv #l #ar (v:validate_with_action_t p inv l ar)
                     #nz' #wk' (k':parser_kind nz' wk'{k' `is_weaker_than` k})
   : Tot (validate_with_action_t (parse_weaken p k') inv l ar)
-  = fun input startPosition ->
-    let h = HST.get () in
-    v input startPosition
+  = fun input ->
+    v input
 
 
 /// Parser: weakening kinds
@@ -650,20 +688,26 @@ let validate_weaken_right (#nz:_) #wk (#k:parser_kind nz wk) (#t:_) (#p:parser k
 inline_for_extraction noextract
 let validate_impos ()
   : Tot (validate_with_action_t (parse_impos ()) true_inv eloc_none true)
-  = fun _ _ -> validator_error_impossible
+  = fun _ -> validator_error_impossible
 
 inline_for_extraction noextract
 let validate_with_error
   c v
-  = fun input startPosition ->
-    let endPositionOrError = v input startPosition in
-    LPL.maybe_set_error_code endPositionOrError startPosition c
+  = fun input ->
+    let h = HST.get () in
+    let startPosition = I.get_read_count input in
+    let startPosition = Cast.uint32_to_uint64 startPosition in
+    let h05 = HST.get () in
+    assert (h05 `extends` h);
+    modifies_address_liveness_insensitive_unused_in h h05;
+    let result = v input in
+    LPL.maybe_set_error_code result startPosition c
 
 noextract inline_for_extraction
 let validate_ite
   e p1 v1 p2 v2
-  = fun input startPosition ->
-      if e then validate_drop (v1 ()) input startPosition else validate_drop (v2 ()) input startPosition
+  = fun input ->
+      if e then validate_drop (v1 ()) input else validate_drop (v2 ()) input
 
 module LPLL = LowParse.Spec.List
 
